Turn tree existence into a type class (but we need a better resolution alg.)

PostComplete/Basic.lean
@@ -81,8 +81,12 @@ lemma test : (λ b ↦ if b then false else true) = not :=
 by
   apply funext; intro b; split <;> simp at * <;> assumption
 
+class HasEval (F : Family) (n : ℕ) (f : Func n) : Type where
+  tree : AppTree F n
+  is_evaltree : evalTree tree = f
+
 -- FIXME: should this be a sigma?
-def CompleteForFN (F G : Family) (n : ℕ) : Prop := ∀ (f : Func n), f ∈ G n → ∃ (t : AppTree F n) , evalTree t = f
+def CompleteForFN (F G : Family) (n : ℕ) : Prop := ∀ (f : Func n), f ∈ G n → (Nonempty $ HasEval F n f)
 
 def Full : Family := λ _ ↦ Set.univ
 
@@ -162,15 +166,17 @@ lemma eval_app_eq {F : Family} (f : Func n) (h : f ∈ F n) :
   evalTree (f_tree f h) = f := by
 simp [evalTree]
 
+#print HasEval
+
 lemma complete_for_n_mon_1 (F F') n : F ⊆ F' → CompleteForN F n → CompleteForN F' n :=
 by
   simp [CompleteForN, CompleteForFN]
   intros sub h f _
   specialize h f _; trivial
   cases h
-  case intro t eq_t =>
-    exists (bumpTree sub t)
-    rw [← eval_bumpTree_eq]; trivial
+  case intro _ t =>
+    exists (bumpTree sub t.tree)
+    rw [← eval_bumpTree_eq]; simp [t.is_evaltree]
 
 #check List.indexOf_get
 
@@ -189,7 +195,7 @@ intros fs _ tree_mem f _
 have f_mem_funclist : f ∈ fs :=
   by apply mem_FuncList
 let i := List.indexOf f fs
-apply Exists.intro (ts.get! i)
+use (ts.get! i)
 have i_lt_len : i < fs.length := by
   exact List.indexOf_lt_length.mpr f_mem_funclist
 rw [← @List.indexOf_get _ _ f]
@@ -267,19 +273,39 @@ lemma eval_mon_complete {F F'} : CompleteForN F' n →
 
 #print AppTree.App
 
+#print HasEval
 
--- This is tedious, can't figure out a way to spell this out...
-def trueSyn : AppTree NAOT 0 :=
-  .App true_n (by simp) unit
+instance hasEvalF F n f (h : f ∈ F n) : HasEval F n f :=
+by
+  use (.App f h (λ i ↦ .Var i))
+  simp [evalTree]
 
-def notSyn (x : AppTree NAOT n) : AppTree NAOT n :=
-  .App not1 (by simp) ![x]
 
-def andSyn (x  y : AppTree NAOT n) : AppTree NAOT n :=
-  .App and2 (by simp) ![x, y]
+instance hasEvalApp0 F f (h : f ∈ F 0) : HasEval F 0 f :=
+by
+  use (.App f h unit)
+  simp [evalTree]
+  apply funext; simp
 
-def orSyn (x  y : AppTree NAOT n) : AppTree NAOT n :=
-  .App or2 (by simp) ![x, y]
+instance hasEvalApp1 F n f (h : f ∈ F 1) (g : Func n) [g_eval : HasEval F n g] : HasEval F n (λ b ↦ f ![g b]) :=
+by
+  use (.App f h ![g_eval.tree])
+  simp [evalTree]
+  apply funext; intros b
+  rw [g_eval.is_evaltree]
+  congr
+  apply funext; simp
+
+
+instance hasEvalApp2 F n f (h : f ∈ F 2) (g₁ g₂ : Func n) [g₁_eval : HasEval F n g₁] [g₂_eval : HasEval F n g₂] : HasEval F n (λ b ↦ f ![g₁ b, g₂ b]) :=
+by
+  use (.App f h ![g₁_eval.tree, g₂_eval.tree])
+  simp [evalTree]
+  apply funext; intros b
+  congr; apply funext; intros i
+  match i with
+  | 0 => simp; rw [g₁_eval.is_evaltree]
+  | 1 => simp; rw [g₂_eval.is_evaltree]
 
 
 lemma complete_NAOT_0 : CompleteForN NAOT 0 := by
@@ -287,19 +313,29 @@ lemma complete_NAOT_0 : CompleteForN NAOT 0 := by
   intros f
   cases h : (f unit)
   case false =>
-    exists (notSyn trueSyn)
-    apply funext; intros x
-    simp [evalTree, not1, true_n]
-    trivial
+    have h' : f = λ b ↦ not1 ![true_n b] :=
+    by
+      apply funext
+      intros x; simp [h, not1, true_n]
+    rw [h']
+    have has_eval_true : HasEval NAOT 0 true_n :=
+      by apply hasEvalF; simp
+    constructor; apply hasEvalApp1; simp
   case true =>
-    exists trueSyn
-    apply funext; intros x
-    simp [evalTree, true_n]; trivial
+    constructor
+    apply hasEvalF; simp
+    apply funext; simp [true_n]; trivial
 
 #check subst
 
 def liftAppTree (t : AppTree F n) : AppTree F (n+1) :=
   subst t (λ i ↦ .Var i)
+
+#check HasEval
+#print inst_fun
+
+instance hasEvalInst [HasEval F (n+1) f] [HasEval F 0 true_n] [HasEval F 0 false_n] : HasEval F n (inst_fun f n k b) :=
+by sorry
 
 theorem complete_NAOT : Complete NAOT :=
 by
@@ -310,11 +346,12 @@ by
     intros f h
     let f_true : Func n := inst_fun f n (by simp) true
     let f_false : Func n := inst_fun f n (by simp) false
-    let tree_f_true := complete_NAOT _ f_true (by simp [Full])
-    let tree_f_false := complete_NAOT _ f_false (by simp [Full])
-    cases tree_f_true
-    cases tree_f_false
-    case intro.intro t_true h₁ t_false h₂ =>
-      exists (orSyn (andSyn (.Var n) (liftAppTree t_true))
-             (andSyn (notSyn (.Var n)) (liftAppTree t_false)))
-      sorry
+    let ⟨ tree_f_true ⟩ := complete_NAOT _ f_true (by simp [Full])
+    let ⟨ tree_f_false ⟩ := complete_NAOT _ f_false (by simp [Full])
+    constructor
+    -- cases tree_f_true
+    -- cases tree_f_false
+    -- case intro.intro t_true h₁ t_false h₂ =>
+    --   exists (orSyn (andSyn (.Var n) (liftAppTree t_true))
+    --          (andSyn (notSyn (.Var n)) (liftAppTree t_false)))
+    sorry
